Progress with Danel

iocy/FancyTraces_Async_Await.fst
@@ -1,20 +1,24 @@
 module FancyTraces_Async_Await
 
 open FStar.Tactics
-open FStar.List.Tot.Base
+open FStar.List.Tot
 open FStar.Classical.Sugar
+open FStar.Ghost
 
-type w_post #e (a:Type) = e -> a -> Type0
-type w_pre #e = e -> Type0
-type w0 #e (a:Type) = w_post #e a -> w_pre #e
+friend Promise
+
+type w_post #s (a:Type) = s -> a -> Type0
+type w_pre #s = s -> Type0
+type w0 #s (a:Type) = w_post #s a -> w_pre #s
 unfold
-let w_post_ord (#e:Type) (#a:Type) (p1 p2:w_post #e a) = forall lt (r:a). p1 lt r ==> p2 lt r
+let w_post_ord (#s:Type) (#a:Type) (p1 p2:w_post #s a) = forall lt (r:a). p1 lt r ==> p2 lt r
 
-let w_monotonic (#e:Type) (#a:Type) (wp:w0 #e a) =
+let w_monotonic (#s:Type) (#a:Type) (wp:w0 #s a) =
   forall (p1 p2:w_post a). (p1 `w_post_ord` p2) ==> (forall h. wp p1 h ==> wp p2 h)
 
-type w (#e:Type) (a:Type) = wp:(w0 #e a){w_monotonic wp}
+type w (#s:Type) (a:Type) = wp:(w0 #s a){w_monotonic wp}
 
+(**
 #push-options "--__no_positivity"
 noeq
 type event (e: Type0) =
@@ -22,6 +26,14 @@ type event (e: Type0) =
 | EAsync : nat -> b:Type0 -> w #(list (event e)) b -> event e
 | EAwait : nat -> event e
 #pop-options
+**)
+
+noeq
+type event (e: Type0) =
+| Ev : e -> event e
+| EAsync : #b:Type0 -> promise b -> trace e -> event e
+| EAwait : #b:Type0 -> promise b -> event e
+and trace e = list (event e)
 
 (** Waiting twice for the same await
 let ex1 =
@@ -60,3 +72,618 @@ let ex3 =
   print 2;
   {{ [1;2];[0;1;2];[1;0;2];[1;2;0] }}
 **)
+let w_equiv (wp1:w 'a) (wp2:w 'a) =
+  forall p h. wp1 p h <==> wp2 p h
+let (≡) = w_equiv
+
+let w_subcomp (#e:Type) (#a:Type) (wp:w a) (p1 p2:w_post a) (h:trace e) :
+  Lemma (requires (wp p1 h /\ p1 `w_post_ord` p2))
+        (ensures (wp p2 h)) = ()
+
+unfold
+let w_ord0 (#s:Type) (#a:Type) (wp1:w #s a) (wp2:w #s a) = forall (p:w_post a) h. wp1 p h ==> wp2 p h
+let w_ord = w_ord0
+unfold let (⊑) = w_ord
+
+unfold
+let w_return0 (#a:Type) (#e:Type) (x:a) : w #(trace e) a =
+  fun p _ -> p [] x
+let w_return = w_return0
+
+unfold
+let w_post_shift (#e:Type) (p:w_post 'b) (lt:trace e) : w_post 'b =
+  fun lt' r' -> p (lt `append` lt') r'
+
+unfold
+let w_post_bind
+  (#e:Type)
+  (#a:Type u#a) (#b:Type u#b)
+  (h:trace e)
+  (kw : a -> w b)
+  (p:w_post b) :
+  Tot (w_post a) =
+  fun lt (x:a) ->
+    kw x (w_post_shift p lt) (h `append` lt) (** Having local trace separate from the history helps with interleavings **)
+
+
+unfold
+let w_bind0 (#e:Type) (#a:Type u#a) (#b:Type u#b) (wp : w a) (kwp : a -> w b) : w b =
+  fun p h -> wp (w_post_bind #e h kwp p) h
+let w_bind = w_bind0
+
+let w_bind_subcomp (wp1:w 'a) (wp2:'a -> w 'b) (wp3:'a -> w 'b) :
+  Lemma
+    (requires ((forall x p h. wp2 x p h <==> wp3 x p h)))
+    (ensures (forall p h. w_bind wp1 wp2 p h <==> w_bind wp1 wp3 p h)) = ()
+
+let __iff_refl a : Lemma (a <==> a) = ()
+let w_law1 (x:'a) (k:'a -> w #(trace 'e) 'b) : Lemma (forall p h. w_bind (w_return x) k p h <==> k x p h) = admit ()
+(**by (
+  norm [delta_only [`%w_bind;`%w_bind0;`%w_return;`%w_return0;`%w_post_bind;`%w_post_shift]; zeta;iota];
+  smt ();
+  dump "H"
+)= ()**)
+
+let w_law2 (m:w 'a) : Lemma (forall p h. w_bind m w_return p h <==> m p h) = admit ()
+let w_law3 (m:w 'a) (g:'a -> w 'b) (k:'b -> w 'c) : Lemma (forall p h. w_bind (w_bind m g) k p h <==> w_bind m (fun x -> w_bind (g x) k) p h) =
+  let lhs = w_bind m (fun r1 -> w_bind (g r1) k) in
+  let rhs = w_bind (w_bind m g) k in
+  let pw (p : w_post 'c) h : Lemma (lhs p h <==> rhs p h) =
+    assert (lhs p h <==> rhs p h) by begin
+      unfold_def (`w_bind);
+      norm [];
+      l_to_r [`List.Tot.Properties.append_assoc];
+      mapply (`__iff_refl)
+    end
+  in
+  Classical.forall_intro_2 pw
+
+noeq
+type free (#e:Type u#0) (a:Type u#a) : Type u#(max 1 a) =
+| Require : (pre:pure_pre) -> k:((squash pre) -> free u#a #e a) -> free #e a
+| Return : a -> free #e a
+| Print : (arg:e) -> cont:(unit -> free u#a #e a) -> free #e a
+| Async : #c:Type u#0 -> free #e (Universe.raise_t u#0 u#a c) -> k:(promise c -> free u#a #e a) -> free #e a
+| Await : #c:Type u#0 -> promise c -> k:(c -> free u#a #e a) -> free #e a
+
+let free_return (#e:Type) (#a:Type) (x:a) : free #e a =
+  Return x
+
+let rec free_bind
+  (#e:Type)
+  (#a:Type u#a)
+  (#b:Type u#b)
+  (l : free #e a)
+  (cont : a -> free #e b) :
+  free #e b =
+  match l with
+  | Require pre k ->
+      Require pre (fun _ -> free_bind (k ()) cont)
+  | Return x -> cont x
+  | Print str k ->
+      Print str (fun i -> free_bind (k i) cont)
+  | Async f k ->
+      Async
+        (free_bind f (fun x -> free_return (Universe.raise_val u#0 u#b (Universe.downgrade_val x))))
+        (fun x -> free_bind (k x) cont)
+  | Await pr k ->
+      Await pr (fun x -> free_bind (k x) cont)
+
+let w_require (pre:pure_pre) : w (squash pre) =
+  let wp' : w0 (squash pre) = fun p h -> pre /\ p [] () in
+  wp'
+
+unfold
+let w_print #e (ev:e) : w unit =
+  fun p _ -> p [Ev ev] ()
+
+unfold let async_event (pr:promise 'a) (asynced_lt:trace 'e) : trace 'e = [EAsync pr asynced_lt]
+
+type wst #s a = s0:nat -> w #s (s1:nat * a) // {s0 <= s1}
+let wst_return #e #a x : wst #(trace e) a = fun s0 -> w_return (s0, x)
+let wst_bind #e #a (m:wst #(trace e) a) #b (k:a -> wst #(trace e) b) : wst #(trace e) b =
+  fun s0 -> w_bind #e #(s1:nat * a) #(s2:nat * b) (m s0) (fun (s1, r) -> k r s1)
+
+unfold let w_async0 (#e:Type0) (#a:Type0) (wf:wst (Universe.raise_t u#0 u#c a)) : wst (promise a) =
+  wst_bind wf (fun r s1 -> w_return #_ #e (s1+1, (Promise (s1+1) (hide (Universe.downgrade_val r)))))
+
+//  fun (s0:nat) -> w_bind (wf s0) (fun (s1r:(nat * _)) -> let (s1, r) = s1r in w_return #(nat * promise a) #e (s1+1, (Promise (s1+1) (hide (Universe.downgrade_val r)))))
+let wst_async #e #a (wf:wst #(trace e) (Universe.raise_t a)) : wst #(trace e) (promise a) =
+  fun s0 p h -> w_async0 wf s0 (fun ltf (s1, pr) -> p (async_event pr ltf) (s1, pr)) h
+
+let w_await (pr:promise 'a) : w 'a =
+  fun p h -> p [EAwait pr] (reveal (Promise?.r pr))
+
+val theta : (#e:Type) -> (#a:Type) -> free #e a -> wst #(trace e) a
+let rec theta m = fun s0 ->
+  match m with
+  | Require pre k ->
+      w_bind (w_require pre) (fun r -> theta (k r) s0)
+  | Return x -> w_return (s0, x)
+  | Print arg k ->
+      w_bind (w_print arg) (fun r -> theta (k r) s0)
+  | Async f k ->
+      w_bind (wst_async (theta f) s0) (fun (s1, pr) -> theta (k pr) s1)
+  | Await pr k ->
+      w_bind (w_await pr) (fun r -> theta (k r) s0)
+
+let theta_monad_morphism_ret (v:'a) (s0:nat) :
+  Lemma (theta (free_return v) s0 == w_return (s0, v)) by (compute ()) = ()
+
+(**
+let lemma_w_async #e #a (wf:w #e (nat * (Universe.raise_t a))) (s0:nat) : Lemma (
+  w_async (s0+1) (w_bind wf (fun (s1,x) -> w_return (s1,(Universe.raise_val (Universe.downgrade_val x)))))
+  ≡
+  w_async (s0+1) wf) by (norm [delta_only [`%w_bind;`%w_bind0;`%w_return;`%w_return0]; iota]) = ()
+
+#set-options "--split_queries always --z3rlimit 10"
+let rec theta_monad_morphism_bind0 (#e:Type) (#a:Type u#a) (#b:Type u#b) (m:free a) (km:a -> free b) (s0:nat) (p:w_post (nat * b)) h :
+  Lemma (w_bind (theta #e m s0) (fun (s1, x) -> theta (km x) s1) p h <==> theta (free_bind m km) s0 p h) =
+  match m with
+  | Return _ -> ()
+  | Require pre k ->
+    calc (<==>) {
+      w_bind (theta #e m s0) (fun (s1, x) -> theta #e (km x) s1) p h;
+      <==> {}
+      w_bind (theta #e (Require pre k) s0) (fun (s1, x) -> theta #e (km x) s1) p h;
+      <==> {}
+      w_bind (w_bind (w_require pre) (fun x -> theta (k x) s0)) (fun (s1, x) -> theta #e (km x) s1) p h;
+      <==> { w_law3 (w_require pre) (fun x ->  theta (k x) s0) (fun (s1, x) -> theta #e (km x) s1) }
+      w_bind (w_require pre) (fun x -> w_bind (theta (k x) s0) (fun (s1, x) -> theta #e (km x) s1)) p h;
+      <==> {
+        let rhs = (fun x -> w_bind (theta (k x) s0) (fun (s1, x) -> theta #e (km x) s1)) in
+        let rhs' = (fun x -> theta (free_bind (k x) km) s0) in
+        introduce forall (x:squash pre) p h. rhs x p h <==> rhs' x p h with
+          theta_monad_morphism_bind0 (k x) km s0 p h;
+        assert (forall x. rhs x p h <==> rhs' x p h);
+        w_bind_subcomp (w_require pre) rhs rhs';
+        assert (w_bind (w_require pre) rhs p h <==> w_bind (w_require pre) rhs' p h)
+       }
+      w_bind (w_require pre) (fun x -> theta (free_bind (k x) km) s0) p h;
+      <==> {}
+      theta #e (Require pre (fun x -> free_bind (k x) km)) s0 p h;
+      <==> {}
+      theta #e (free_bind (Require pre k) km) s0 p h;
+      <==> {}
+      theta #e (free_bind m km) s0 p h;
+    }
+  | Print arg k ->
+    calc (<==>) {
+      w_bind (theta #e m s0) (fun (s1, x) -> theta #e (km x) s1) p h;
+      <==> {}
+      w_bind (theta #e (Print arg k) s0) (fun (s1, x) -> theta #e (km x) s1) p h;
+      <==> {}
+      w_bind (w_bind (w_print arg) (fun x -> theta (k x) s0)) (fun (s1, x) -> theta #e (km x) s1) p h;
+      <==> { w_law3 (w_print arg) (fun x ->  theta (k x) s0) (fun (s1, x) -> theta #e (km x) s1) }
+      w_bind (w_print arg) (fun x -> w_bind (theta (k x) s0) (fun (s1, x) -> theta #e (km x) s1)) p h;
+      <==> {
+        let rhs = (fun x -> w_bind (theta (k x) s0) (fun (s1, x) -> theta #e (km x) s1)) in
+        let rhs' = (fun x -> theta (free_bind (k x) km) s0) in
+        introduce forall x p h. rhs x p h <==> rhs' x p h with
+          theta_monad_morphism_bind0 (k x) km s0 p h;
+        assert (forall x. rhs x p h <==> rhs' x p h);
+        w_bind_subcomp (w_print arg) rhs rhs';
+        assert (w_bind (w_print arg) rhs p h <==> w_bind (w_print arg) rhs' p h)
+       }
+      w_bind (w_print arg) (fun x -> theta (free_bind (k x) km) s0) p h;
+      <==> {}
+      theta #e (Print arg (fun x -> free_bind (k x) km)) s0 p h;
+      <==> {}
+      theta #e (free_bind (Print arg k) km) s0 p h;
+      <==> {}
+      theta #e (free_bind m km) s0 p h;
+    }
+  | Await pr k ->
+    calc (<==>) {
+      w_bind (theta #e m s0) (fun (s1, x) -> theta #e (km x) s1) p h;
+      <==> {}
+      w_bind (theta #e (Await pr k) s0) (fun (s1, x) -> theta #e (km x) s1) p h;
+      <==> {}
+      w_bind (w_bind (w_await pr) (fun x -> theta (k x) s0)) (fun (s1, x) -> theta #e (km x) s1) p h;
+      <==> { w_law3 (w_await pr) (fun x ->  theta (k x) s0) (fun (s1, x) -> theta #e (km x) s1) }
+      w_bind (w_await pr) (fun x -> w_bind (theta (k x) s0) (fun (s1, x) -> theta #e (km x) s1)) p h;
+      <==> {
+        let rhs = (fun x -> w_bind (theta (k x) s0) (fun (s1, x) -> theta #e (km x) s1)) in
+        let rhs' = (fun x -> theta (free_bind (k x) km) s0) in
+        introduce forall x p h. rhs x p h <==> rhs' x p h with
+          theta_monad_morphism_bind0 (k x) km s0 p h;
+        assert (forall x. rhs x p h <==> rhs' x p h);
+        w_bind_subcomp (w_await pr) rhs rhs';
+        assert (w_bind (w_await pr) rhs p h <==> w_bind (w_await pr) rhs' p h)
+       }
+      w_bind (w_await pr) (fun x -> theta (free_bind (k x) km) s0) p h;
+      <==> {}
+      theta #e (Await pr (fun x -> free_bind (k x) km)) s0 p h;
+      <==> {}
+      theta #e (free_bind (Await pr k) km) s0 p h;
+      <==> {}
+      theta #e (free_bind m km) s0 p h;
+    }
+  | Async f k ->
+    calc (<==>) {
+      w_bind (theta #e m s0) (fun (s1, x) -> theta #e (km x) s1) p h;
+      <==> {}
+      w_bind (theta #e (Async f k) s0) (fun (s1, x) -> theta #e (km x) s1) p h;
+      <==> {}
+      w_bind (w_bind (w_async (s0+1) (theta f (s0+1))) (fun (s1, x) -> theta (k x) s1)) (fun (s2, x) -> theta #e (km x) s2) p h;
+      <==> { w_law3 (w_async (s0+1) (theta f (s0+1))) (fun (s1, x) ->  theta (k x) s1) (fun (s2, x) -> theta #e (km x) s2) }
+      w_bind (w_async (s0+1) (theta f (s0+1))) (fun (s1, x) -> w_bind (theta (k x) s1) (fun (s2, x) -> theta #e (km x) s2)) p h;
+      <==> {
+        let rhs = (fun (s1, x) -> w_bind (theta (k x) s1) (fun (s2, x) -> theta #e (km x) s2)) in
+        let rhs' = (fun (s1, x) -> theta (free_bind (k x) km) s1) in
+        introduce forall x s0 p h. rhs (s0,x) p h <==> rhs' (s0,x) p h with
+          theta_monad_morphism_bind0 (k x) km s0 p h;
+        assert (forall x. rhs x p h <==> rhs' x p h);
+        w_bind_subcomp (w_async (s0+1) (theta f (s0+1))) rhs rhs';
+        assert (w_bind (w_async (s0+1) (theta f (s0+1))) rhs p h <==> w_bind (w_async (s0+1) (theta f (s0+1))) rhs' p h)
+       }
+      w_bind (w_async (s0+1) (theta f (s0+1))) (fun (s1, x) -> theta (free_bind (k x) km) s1) p h;
+      <==> { lemma_w_async (theta f (s0+1)) s0 }
+      w_bind (w_async (s0+1) (w_bind (theta f (s0+1)) (fun (s1,x) -> w_return (s1,(Universe.raise_val (Universe.downgrade_val x))))))
+           (fun (s1, x) -> theta (free_bind (k x) km) s1) p h;
+      <==> { _ by (norm [delta_only [`%free_return]; iota]) }
+      w_bind (w_async (s0+1) (w_bind (theta f (s0+1)) (fun (s1,x) -> theta (free_return (Universe.raise_val (Universe.downgrade_val x))) s1)))
+           (fun (s1, x) -> theta (free_bind (k x) km) s1) p h;
+      <==> {
+        let k = (fun x -> free_return (Universe.raise_val (Universe.downgrade_val x))) in
+        introduce forall s0 p h. w_bind (theta #e f s0) (fun (s1, x) -> theta #e (k x) s1) p h <==> theta #e (free_bind f k) s0 p h with
+          theta_monad_morphism_bind0 f k s0 p h }
+      w_bind (w_async (s0+1) (theta ((free_bind f (fun x -> free_return (Universe.raise_val (Universe.downgrade_val x))))) (s0+1))) (fun (s1, x) -> theta (free_bind (k x) km) s1) p h;
+      <==> {}
+      theta (Async (free_bind f (fun x -> free_return (Universe.raise_val (Universe.downgrade_val x)))) (fun x -> free_bind (k x) km)) s0 p h;
+      <==> { _ by (compute ()) }
+      theta #e (free_bind (Async f k) km) s0 p h;
+      <==> {}
+      theta #e (free_bind m km) s0 p h;
+    }
+#reset-options
+
+let theta_monad_morphism_bind (#e:Type) (#a:Type) (#b:Type) (m:free a) (km:a -> free b) :
+  Lemma (forall s0. w_bind (theta #e m s0) (fun (s1, x) -> theta (km x) s1) ≡ theta (free_bind m km) s0) =
+  Classical.forall_intro_3 (theta_monad_morphism_bind0 m km)
+
+**)
+
+let theta' m s0 = w_bind (theta m s0) (fun (s1, x) -> w_return x)
+
+let lemma_wp_drop_state (wp:w #(trace 'e) (nat * 'a)) p h : Lemma (
+   w_bind wp (fun (_, x) -> w_return x) p h <==> wp (fun lt (_, rf) -> p lt rf) h) = admit ()
+
+let lemma_theta_theta'0 (m:free #'e 'a) s0 p h : Lemma (
+   theta' m s0 p h <==> theta m s0 (fun lt (s1, rf) -> p lt rf) h) =
+   lemma_wp_drop_state (theta m s0) p h
+
+let lemma_theta_theta' (m:free #'e 'a) : Lemma (
+   forall s0 p h. theta' m s0 p h <==> theta m s0 (fun lt (s1, rf) -> p lt rf) h) =
+   Classical.forall_intro_3 (lemma_theta_theta'0 m)
+
+let dm (#e:Type0) (a:Type u#a) (wp:w #(trace e) a) =
+  m:(free a){forall s0. wp ⊑ theta' m s0}
+
+let dm_return (a:Type u#a) (x:a) : dm a (w_return0 x) =
+  Return x
+
+(**
+let lemma_better_sub0
+  (#e:Type)
+  (#a:Type u#a)
+  (#b:Type u#b)
+  (wp:w #e a)
+  (kwp:a -> w #e b)
+  (c:dm a wp)
+  (kc:(x:a -> dm b (kwp x)))
+  (s0:nat)
+  (p:w_post #e b)
+  h : Lemma
+    (requires (
+      let p1' : w_post #e (nat * a) = (fun lt (s1, x) -> theta (kc x) s1 (w_post_shift (fun lt' (_, x') -> p lt' x') lt) (append h lt)) in
+      theta c s0 p1' h))
+    (ensures (w_bind (w_bind (theta c s0) (fun (s1, x) -> theta (kc x) s1)) (fun (_, x) -> w_return x) p h)) =
+  calc (==>) {
+    theta c s0 (fun lt (s1, x) -> theta (kc x) s1 (w_post_shift (fun lt' (_, x') -> p lt' x') lt) (append h lt)) h;
+    ==> { _ by (norm [delta_only [`%w_bind; `%w_bind0]; iota]) }
+    w_bind (theta c s0) (fun (s1, x) -> theta (kc x) s1) (fun lt (_, x) -> p lt x) h;
+    ==> { lemma_wp_drop_state (w_bind (theta c s0) (fun (s1, x) -> theta (kc x) s1)) p h }
+    w_bind (w_bind (theta c s0) (fun (s1, x) -> theta (kc x) s1)) (fun (_, x) -> w_return x) p h;
+  }
+
+let lemma_better
+  (#e:Type)
+  (#a:Type u#a)
+  (#b:Type u#b)
+  (wp:w #e a)
+  (kwp:a -> w #e b)
+  (c:dm a wp)
+  (kc:(x:a -> dm b (kwp x))) : Lemma
+    (requires ((forall s0. wp ⊑ w_bind (theta c s0) (fun (_, x) -> w_return x)) /\
+              (forall s0 x. kwp x ⊑ w_bind (theta (kc x) s0) (fun (_, x) -> w_return x))))
+    (ensures (forall s0. w_bind wp kwp ⊑ w_bind (w_bind (theta c s0) (fun (s1, x) -> theta (kc x) s1)) (fun (_, x) -> w_return x))) =
+  introduce forall s0 (p:w_post b) h. w_bind wp kwp p h ==> w_bind (w_bind (theta c s0) (fun (s1, x) -> theta (kc x) s1)) (fun (_, x) -> w_return x) p h with begin
+    introduce w_bind wp kwp p h ==> w_bind (w_bind (theta c s0) (fun (s1, x) -> theta (kc x) s1)) (fun (_, x) -> w_return x) p h with _. begin
+      let p1' : w_post #e (nat * a) = (fun lt (s1, x) -> theta (kc x) s1 (w_post_shift (fun lt' (_, x') -> p lt' x') lt) (append_runtree h lt)) in
+      let _ : squash (theta c s0 p1' h) = begin
+        eliminate forall s0. wp ⊑ w_bind (theta c s0) (fun (_, x) -> w_return x) with s0;
+        assert (forall (p':w_post #e a) h. wp p' h ==> w_bind (theta c s0) (fun (_, x) -> w_return x) p' h);
+        let p0 : w_post #e a = fun lt x -> kwp x (w_post_shift p lt) (append_runtree h lt) in
+        assert (wp p0 h);
+        let p0' : w_post #e a = fun lt x -> forall s1. theta (kc x) s1 (w_post_shift (fun lt' (_, x') -> p lt' x') lt) (append_runtree h lt) in
+        introduce forall lt x. p0 lt x ==> p0' lt x with begin
+            assert (forall p h s1 x. kwp x p h ==> w_bind (theta (kc x) s1) (fun (_, x) -> w_return x) p h);
+            assert (forall p h x. kwp x p h ==> (forall s1. w_bind (theta (kc x) s1) (fun (_, x) -> w_return x) p h));
+            let p' : w_post #e b = w_post_shift p lt in
+            let h' = (append_runtree h lt) in
+            eliminate forall p h x. kwp x p h ==> (forall s1. w_bind (theta (kc x) s1) (fun (_, x) -> w_return x) p h) with p' h' x;
+            introduce p0 lt x ==> p0' lt x with _. begin
+            assert (kwp x p' h');
+            assert (forall s1. w_bind (theta (kc x) s1) (fun (_, x) -> w_return x) p' h');
+            introduce forall s1. theta (kc x) s1 (fun lt (_, x) -> p' lt x) h' with
+                lemma_theta_theta'0 (kc x) s1 p' h';
+            assert (p0' lt x)
+            end
+        end;
+        assert (wp p0' h);
+        eliminate forall (p':w_post #e a) h. wp p' h ==> w_bind (theta c s0) (fun (_, x) -> w_return x) p' h with p0' h;
+        assert (w_bind (theta c s0) (fun (_, x) -> w_return x) p0' h);
+        let p1 : w_post #e (nat * a) = (fun lt (_, x) -> p0' lt x) in
+        lemma_theta_theta'0 c s0 p0' h;
+        assert (theta c s0 p1 h);
+        assert (p1 `w_post_ord` p1');
+        w_subcomp (theta c s0) p1 p1' h;
+        assert (theta c s0 p1' h)
+      end in
+
+      lemma_better_sub0 wp kwp c kc s0 p h
+    end
+  end
+**)
+
+let dm_bind
+  (#e:Type)
+  (a:Type u#a)
+  (b:Type u#b)
+  (wp:w #(trace e) a)
+  (kwp:a -> w #(trace e) b)
+  (c:dm a wp)
+  (kc:(x:a -> dm b (kwp x))) :
+  dm #e b (w_bind0 wp kwp) =
+  let m = free_bind c kc in
+  admit ();
+ // lemma_better wp kwp c kc;
+ // theta_monad_morphism_bind c kc;
+ // assert (forall s0. w_bind (theta c s0) (fun (s1, x) -> theta (kc x) s1) ⊑ theta m s0);
+ // assert (forall s0. w_bind wp kwp ⊑ theta' m s0);
+  m
+
+let dm_subcomp
+  (#e:Type)
+  (a:Type u#a)
+  (wp1:w #(trace e) a)
+  (wp2:w #(trace e) a)
+  (c:dm a wp1) :
+  Pure (dm a wp2)
+    (requires (wp2 `w_ord0` wp1))
+    (ensures (fun _ -> True)) =
+    c
+
+let w_if_then_else (#e:Type) (#a:Type) (wp1 wp2:w #e a) (b:bool) : w #e a =
+  fun p h -> (b ==> wp1 p h) /\ ((~b) ==> wp2 p h)
+
+let dm_if_then_else (#e:Type) (a : Type u#a)
+  (wp1 wp2: w #(trace e) a) (f : dm a wp1) (g : dm a wp2) (b : bool) : Type =
+  dm a (w_if_then_else wp1 wp2 b)
+
+let dm_partial_return
+  (#e:Type)
+  (pre:pure_pre) : dm #e (squash pre) (w_require pre) =
+  let m = Require pre (Return) in
+  assert (forall s0. w_require pre ⊑ theta' #e m s0) by (compute ());
+  m
+
+unfold
+let lift_pure_w (#e:Type0) (#a:Type u#a) (wp : pure_wp a) : w #(trace e) a =
+  FStar.Monotonic.Pure.elim_pure_wp_monotonicity_forall ();
+  (fun (p:w_post a) _ -> wp (fun (r:a) -> p [] r))
+
+let lift_pure_w_as_requires (#e:Type) (#a:Type) (wp : pure_wp a) :
+  Lemma (forall (p:w_post #(trace e) a) h. lift_pure_w wp p h ==> as_requires wp) =
+    assert (forall (p:w_post #(trace e) a) x. p [] x ==> True) ;
+    FStar.Monotonic.Pure.elim_pure_wp_monotonicity wp;
+    assert (forall (p:w_post #(trace e) a). wp (fun x -> p [] x) ==> wp (fun _ -> True))
+
+reflectable
+reifiable
+total
+effect {
+  CyWP (a:Type) (wp : w #(trace int) a)
+  with {
+       repr       = dm #int
+     ; return     = dm_return #int
+     ; bind       = dm_bind #int
+     ; subcomp    = dm_subcomp #int
+     ; if_then_else = dm_if_then_else #int
+     }
+}
+
+let lift_pure_dm
+  (a : Type u#a)
+  (wp : pure_wp a)
+  (f:(eqtype_as_type unit -> PURE a wp)) :
+  dm #int a (lift_pure_w wp) =
+  lift_pure_w_as_requires #int #a wp;
+  FStar.Monotonic.Pure.elim_pure_wp_monotonicity_forall ();
+  let lhs = dm_partial_return (as_requires wp) in
+  let rhs = (fun (pre:(squash (as_requires wp))) -> dm_return a (f ())) in
+  let m = dm_bind _ _ _ _ lhs rhs in
+  dm_subcomp a _ (lift_pure_w wp) m
+
+sub_effect PURE ~> CyWP = lift_pure_dm
+
+effect Cy
+  (a:Type)
+  (pre : trace int -> Type0)
+  (post : trace int -> a -> trace int -> Type0) =
+  CyWP a (fun p h -> pre h /\ (forall lt r. post h r lt ==> p lt r))
+
+(** *** Tests partiality of the effect **)
+let test_using_assume (fd:int) : Cy int (requires (fun h -> True)) (ensures fun h r lt -> fd % 2 == 0) =
+  assume (fd % 2 == 0) ;
+  fd
+
+// A second test to make sure exfalso isn't used
+let test_assume #a #pre (f : unit -> Cy a (requires (fun _ -> pre)) (ensures fun _ _ _ -> True)) : Cy a (fun _ -> True) (fun _ _ _ -> True) =
+  assume pre ;
+  f ()
+
+let test_assert p : Cy unit (requires (fun _ -> p)) (ensures fun _ _ _ -> True) =
+  assert p
+
+let partial_match (l : list nat) : Cy unit (requires (fun _ -> l <> [])) (ensures fun _ _ _ -> True) =
+  match l with
+  | x :: r -> ()
+
+let partial_match_io (l : list int) : Cy int (requires fun _ -> l <> []) (ensures fun _ _ _ -> True) =
+  match l with
+  | s :: _ -> s + 10
+
+// Cezar's tests
+
+assume val p : prop
+assume val p' : prop
+assume val pure_lemma (_ : unit) : Lemma p
+assume val some_f (_ : squash p) : Cy unit (requires fun _ -> True) (ensures fun _ _ _ -> True)
+assume val some_f' : unit -> Cy unit (requires fun _ -> p) (ensures fun _ _ _ -> p')
+
+// TODO: why is this failing?
+let pure_lemma_test () : Cy unit (requires fun _ -> True) (ensures fun _ _ _ -> True) =
+  pure_lemma () ;
+  some_f ()
+
+let pure_lemma_test2 () : Cy unit (requires fun _ -> True) (ensures fun _ _ _ -> True) =
+  pure_lemma () ;
+  some_f () ;
+  some_f' () ;
+  assert p'
+(** *** DONE with tests of partiality **)
+
+let print (e:int) : Cy unit (fun _ -> True) (fun _ () lt -> lt == return_runtree [Ev e]) =
+  CyWP?.reflect (Print e (Return))
+
+let raise_w (#a:Type u#a) (wp:w a) : w (Universe.raise_t u#a u#b a) =
+  fun p -> wp (fun lt r -> p lt (Universe.raise_val r))
+
+[@"opaque_to_smt"]
+let async00 (#a:Type u#a) (#wp:w a) ($f:unit -> CyWP a wp) : dm (Universe.raise_t u#a u#b a) (raise_w u#a u#b wp)  =
+  let f' : dm a wp = reify (f ()) in
+  dm_subcomp _ _ _ (dm_bind _ _ _ _ f' (fun x -> dm_return _ (Universe.raise_val u#a u#b x)))
+
+let async_spec_implies_theta
+  (#a:Type)
+  (pre:w_pre) (post:tracetree int -> a -> tracetree int -> Type0)
+  (f:dm (Universe.raise_t a) (fun p h -> pre h /\ (forall r lt. post h r lt ==> p lt (Universe.raise_val r)))) :
+  Lemma (
+    forall s0.
+    (fun p h -> pre h /\ (forall pr lt. post h (Promise?.r pr) lt ==> p (async_runtree (Promise?.id pr) lt) pr))
+    ⊑
+    theta' (Async f free_return) s0) =
+  introduce forall s0 (p:w_post (promise a)) h. (pre h /\ (forall pr lt. post h (Promise?.r pr) lt ==> p (async_runtree (Promise?.id pr) lt) pr) ==>
+       theta' (Async f free_return) s0 p h) with begin
+       introduce (pre h /\ (forall pr lt. post h (Promise?.r pr) lt ==> p (async_runtree (Promise?.id pr) lt) pr)) ==>
+       theta' (Async f free_return) s0 p h with hyp. begin
+         let p' : w_post (Universe.raise_t a) = (fun ltf rf -> p (async_runtree (s0+1) ltf) (Promise (s0+1) (Universe.downgrade_val rf))) in
+         let _:squash (theta f (s0+1) (fun ltf (s1, rf) -> p' ltf rf) h) = begin
+            assert (forall (p':w_post (Universe.raise_t a)). pre h /\ (forall r lt. post h r lt ==> p' lt (Universe.raise_val r)) ==> theta' f (s0+1) p' h);
+            lemma_theta_theta' f;
+            assert (forall s0 p h. theta' f s0 p h <==> theta f s0 (fun lt (s1, rf) -> p lt rf) h);
+            eliminate forall p'. pre h /\ (forall r lt. post h r lt ==> p' lt (Universe.raise_val r)) ==> theta f (s0+1) (fun lt (s1, rf) -> p' lt rf) h with p';
+            introduce forall r lt. post h r lt ==> p' lt (Universe.raise_val r) with begin
+              eliminate forall pr. (forall lt. post h (Promise?.r pr) lt ==> p (async_runtree (Promise?.id pr) lt) pr) with (Promise (s0+1) r);
+              eliminate forall lt. post h r lt ==> p (async_runtree (s0+1) lt) (Promise (s0+1) r) with lt
+            end;
+            assert (theta f (s0+1) (fun ltf (s1, rf) -> p' ltf rf) h)
+         end in
+         let _:squash (theta (Async f free_return) s0 (fun lt (s1, pr) -> p lt pr) h) = begin
+            calc (==>) {
+            theta f (s0+1) (fun ltf (s1, rf) -> p' ltf rf) h;
+            ==> { }
+            theta f (s0+1) (fun ltf (s1, rf) -> p (async_runtree (s0+1) ltf) (Promise (s0+1) (Universe.downgrade_val rf))) h;
+            ==> { _ by (norm [delta_only [`%append_runtree;`%empty_runtree]; zeta; iota]; assumption ())}
+            theta f (s0+1) (fun lt (s1, rf) -> p (async_runtree (s0+1) (append_runtree lt empty_runtree)) (Promise (s0+1) (Universe.downgrade_val rf))) h;
+            ==> { _ by (norm [delta_only [`%w_return;`%w_return0]; iota]; assumption ())}
+            theta f (s0+1) (fun lt (s1, rf) -> w_return (s1, Promise (s0+1) (Universe.downgrade_val rf))
+                  (fun lt' (_, pr) -> p (async_runtree (s0+1) (append_runtree lt lt')) pr) (append_runtree h lt)) h;
+            ==> { _ by (norm [delta_only [`%w_async0;`%w_bind;`%w_bind0;`%w_post_bind;`%w_post_shift]; zeta;iota]) }
+            w_async0 (s0+1) (theta f (s0+1)) (fun ltf (s1, pr) -> p (async_runtree (s0+1) ltf) pr) h;
+            ==> { _ by (norm [delta_only [`%w_async]; zeta;iota]; assumption ()) }
+            w_async (s0+1) (theta f (s0+1)) (fun lt (s1, pr) -> p lt pr) h;
+            ==> { _ by (norm [delta_only [`%append_runtree;`%empty_runtree]; zeta; iota]; assumption ())}
+            w_async (s0+1) (theta f (s0+1)) (fun lt (s1, pr) ->
+               p (lt `append_runtree` empty_runtree) pr) h;
+            ==> { _ by (norm [delta_only [`%w_return;`%w_return0]; iota]; assumption ())}
+            w_async (s0+1) (theta f (s0+1)) (fun lt (s1, pr) ->
+              w_return (s1, pr) (fun lt' (_, pr) -> p (lt `append_runtree` lt') pr) (h `append_runtree` lt)) h;
+            ==> { _ by (norm [delta_only [`%w_bind;`%w_bind0;`%w_post_bind;`%w_post_shift]; iota])}
+            w_bind (w_async (s0+1) (theta f (s0+1))) (fun (s1, pr) ->
+              w_return (s1, pr)) (fun lt (s1, pr) -> p lt pr) h;
+            ==> {}
+            w_bind (w_async (s0+1) (theta f (s0+1))) (fun (s1, pr) ->
+              theta (Return pr) s1) (fun lt (s1, pr) -> p lt pr) h;
+            ==> {}
+            w_bind (w_async (s0+1) (theta f (s0+1))) (fun (s1, pr) ->
+              theta (free_return pr) s1) (fun lt (s1, pr) -> p lt pr) h;
+            ==> { _ by (norm [delta_only [`%theta]; zeta;iota]; assumption ()) }
+            theta (Async f free_return) s0 (fun lt (s1, pr) -> p lt pr) h;
+            }
+         end in
+         let _:squash (theta' (Async f free_return) s0 p h) = begin
+           lemma_theta_theta' (Async f free_return)
+         end in
+         assert (theta' (Async f free_return) s0 p h)
+       end
+  end
+
+let async0 (#a:Type) (#pre:w_pre) (#post:tracetree int -> a -> tracetree int -> Type0) ($f:unit -> Cy a pre post) :
+  dm (promise a) (fun p h -> pre h /\ (forall pr lt. post h (Promise?.r pr) lt ==> p (async_runtree (Promise?.id pr) lt) pr)) =
+  let wp' : w (Universe.raise_t a) = raise_w (fun p h -> pre h /\ (forall lt r. post h r lt ==> p lt r)) in
+  let f' : dm (Universe.raise_t a) wp' = async00 f in
+  let m : free (promise a) = Async f' free_return in
+  async_spec_implies_theta pre post f';
+  m
+
+[@"opaque_to_smt"]
+let async (#a:Type) (#pre:w_pre) (#post:tracetree int -> a -> tracetree int -> Type0) ($f:unit -> Cy a pre post) :
+  Cy (promise a) pre (fun h pr lt -> exists lt'. lt == async_runtree (Promise?.id pr) lt' /\ post h (Promise?.r pr) lt') =
+  CyWP?.reflect (async0 f)
+
+[@"opaque_to_smt"]
+let await (#a:Type) (pr:promise a) : Cy a (fun _ -> True) (fun h r lt -> reveal (Promise?.r pr) == r /\ lt == return_runtree [EAwait (Promise?.id pr)]) =
+  CyWP?.reflect (Await pr (free_return))
+
+let return (#a:Type) (x:a) () : Cy a (fun _ -> True) (fun h r lt -> r == x /\ lt == return_runtree [Ev 0;Ev 1;Ev 2]) = print 0; print 1; print 2; x
+
+let test () : Cy int (fun _ -> True) (fun h r lt -> exists (id1 id2:nat). r == 1 /\ lt == Node [EAsync id1] (Node [Ev 0; Ev 1; Ev 2] Leaf Leaf) (Node [EAsync id2] (Node [Ev 0; Ev 1; Ev 2] Leaf Leaf) (Node [Ev 1; Ev 2; Ev 2] Leaf Leaf))) =
+  let prx = async (return 2) in
+  let pry = async (return 3) in
+  print 1;
+  print 2;
+  (if false then print 3
+  else print 2);
+  1
+
+let test2 () : Cy int (fun _ -> True) (fun h r lt -> exists (id1 id2:nat). r == 5 /\ lt == Node [EAsync id1] (Node [Ev 0; Ev 1; Ev 2] Leaf Leaf) (Node [EAsync id2] (Node [Ev 0; Ev 1; Ev 2] Leaf Leaf) (Node [EAwait id1; EAwait id2] Leaf Leaf))) =
+  let prx = async (return 2) in
+  let pry = async (return 3) in
+  let x : int = await prx in
+  let y : int = await pry in
+  x + y
+
+
+let f () : Cy (promise unit) (fun _ -> True) (fun h pr lt -> lt == Node [EAsync (Promise?.id pr)] (Node [Ev 0; Ev 1; Ev 2] Leaf Leaf) Leaf) =
+  async (return ())
+
+let g () : Cy (promise unit)  (fun _ -> True) (fun h pr lt -> lt == Node [Ev 10; EAsync (Promise?.id pr)] (Node [Ev 0; Ev 1; Ev 2] Leaf Leaf) Leaf) =
+  print 10;
+  f ()
+
+let h () : Cy unit (fun _ -> True) (fun h r lt -> exists (id1:nat). lt == Node [Ev 10; EAsync id1] (Node [Ev 0; Ev 1; Ev 2] Leaf Leaf) (Node [EAwait id1; Ev 20] Leaf Leaf)) =
+  await (g ());
+  print 20
